Working on migrating stuff from web-server into main branch.

src/coq/Basis.v
@@ -32,17 +32,82 @@ Require Import Ynot.Hprop.
 
 Require Import String.
 Require Import List.
+Require Import Ascii.
 
 Open Local Scope hprop_scope.
 
+(** String <-> List Conversion **)
+Fixpoint str2la (str : string) : list ascii :=
+  match str with
+    | EmptyString => nil
+    | String a b => a :: (str2la b)
+  end.
+
+Fixpoint la2str (la : list ascii) : string :=
+  match la with
+    | nil => EmptyString
+    | a :: b => String a (la2str b)
+  end.
+
+Theorem str2la_inv_la2str : forall str, la2str (str2la str) = str.
+  induction str; [ auto | simpl; rewrite IHstr; trivial ].
+Qed.
+
+Theorem la2str_inv_str2la : forall str, str2la (la2str str) = str.
+  induction str; [ auto | simpl; rewrite IHstr; trivial ].
+Qed.
+
+(** Standard "println" **)
 Axiom printString : forall (s : string),
   STsep (__) (fun _:unit => __).
 
-Axiom printStringLn : forall (s : string),
-  STsep (__) (fun _:unit => __).
+Definition printStringLn (s : string) :
+  STsep (__) (fun _:unit => __) :=
+  printString (s ++ (String "010"%char (String "013"%char ""%string))).
 
-Axiom printString' : forall (s : list Ascii.ascii),
-  STsep (__) (fun _:unit => __).
+Definition printString' (s : list ascii) :
+  STsep (__) (fun _:unit => __) :=
+  printString (la2str s).
 
-Axiom printStringLn' : forall (s : list Ascii.ascii),
-  STsep (__) (fun _:unit => __).
+Definition printStringLn' (s : list Ascii.ascii) :
+  STsep (__) (fun _:unit => __) :=
+  printStringLn (la2str s).
+
+(** Numbers -> Strings **)
+
+Open Local Scope char_scope.
+
+Definition dd n :=
+  match n with
+    | 0 => "0" | 1 => "1" | 2 => "2" | 3 => "3" | 4 => "4"
+    | 5 => "5" | 6 => "6" | 7 => "7" | 8 => "8" | 9 => "9"
+    | _ => "x"
+  end.
+
+ Fixpoint div_mod_10 (a q : nat) {struct a} :=
+   match a with
+     | 0 => (q,0)
+     | 1 => (q,1)
+     | 2 => (q,2)
+     | 3 => (q,3)
+     | 4 => (q,4)
+     | 5 => (q,5)
+     | 6 => (q,6)
+     | 7 => (q,7)
+     | 8 => (q,8)
+     | 9 => (q,9)
+     | S (S (S (S (S (S (S (S (S (S n))))))))) => div_mod_10 n (S q)
+   end.
+
+ Fixpoint ntos (x : nat) (n : nat) (l : list ascii) {struct x} :=
+   match n with
+     | 0 => match l with
+              | nil => "0" :: l
+              | _ => l
+            end
+     | _ => let (q,r) := div_mod_10 n 0 in
+       match x with
+         | 0 => "t" :: "o" :: "o" ::" " :: "b" :: "i" :: "g" :: nil
+         | S x' => ntos x' q (dd r :: l)
+       end
+   end.
