examples/IO/Net.v
@@ -1,0 +1,121 @@
+Require Import Ynot.
+Require Import IO FS.
+Require Import List Ascii.
+
+Set Implicit Arguments.
+
+Open Local Scope stsepi_scope.
+Open Local Scope hprop_scope.
+
+(** Socket Address **)
+Axiom axiom_SockAddr : Set.
+Definition SockAddr := axiom_SockAddr.
+
+(** constructor for socket addresses **)
+Axiom axiom_sockaddr : forall (n1 n2 n3 n4 : sig (fun x : nat => x <= 255))
+  (port : nat),
+  STsep (__)
+        (fun r : SockAddr => hprop_empty).
+Definition sockaddr := axiom_sockaddr.
+
+Axiom axiom_sock_eq : forall (sa1 sa2 : SockAddr), {sa1 = sa2} + {sa1 <> sa2}.
+Definition sock_eq := axiom_sock_eq.
+
+(** UDP Sockets **)
+Axiom axiom_UDP_Sent : SockAddr -> SockAddr -> list ascii -> Action.
+Axiom axiom_UDP_Recd : SockAddr -> SockAddr -> list ascii -> Action.
+Axiom axiom_UDP_send : forall (local remote: SockAddr) (s: list ascii) (tr: [Trace]),
+  STsep (tr ~~ traced tr)
+        (fun r:unit => tr ~~ traced (axiom_UDP_Sent local remote s :: tr)).   
+Axiom axiom_UDP_recv : forall (local: SockAddr) (tr: [Trace]),
+  STsep (tr ~~ traced tr) 
+        (fun r => tr ~~  traced (axiom_UDP_Recd local (fst r) (snd r) :: tr)).
+
+Module UDP.
+
+  Definition Sent := axiom_UDP_Sent.
+  Definition Recd := axiom_UDP_Recd.
+
+  Definition send : forall (local remote: SockAddr) (s: list ascii) (tr: [Trace]),
+    STsep (tr ~~ traced tr)
+          (fun r:unit => tr ~~ traced (Sent local remote s :: tr)) :=
+    axiom_UDP_send.  
+  Definition recv : forall (local: SockAddr) (tr: [Trace]),
+    STsep (tr ~~ traced tr) 
+          (fun r => tr ~~  traced (Recd local (fst r) (snd r) :: tr)) :=
+    axiom_UDP_recv.
+
+End UDP.
+
+(** TCP Sockets **)
+Axiom axiom_BoundSocketModel : SockAddr -> SockAddr -> fd_model.
+Definition BoundSocketModel := axiom_BoundSocketModel.
+Axiom axiom_ListenSocketModel : SockAddr -> fd_model.
+Definition ListenSocketModel := axiom_ListenSocketModel.
+
+Axiom axiom_TCP_Accept : SockAddr -> SockAddr -> SockAddr -> Action.
+
+Axiom axiom_TCP_listenSocket : forall (skt : SockAddr),
+  STsep (__)
+        (fun fd:(File (ListenSocketModel skt) (R :: nil)) => handle fd).
+
+Definition rt := sigT (fun x:(SockAddr * SockAddr) => (File (BoundSocketModel (fst x) (snd x)) (R :: W :: nil))).
+
+Axiom axiom_TCP_bindSocket : forall (local remote : SockAddr),
+  STsep (__)
+        (fun fd:File (BoundSocketModel local remote) (R :: W :: nil) => handle fd).
+
+Axiom axiom_TCP_accept : forall (skt : SockAddr) (fd : File (ListenSocketModel skt) (R :: nil))
+  (tr : [Trace]),
+  STsep (tr ~~ traced tr)
+        (fun r:rt => tr ~~ handle (projT2 r) *
+            traced (axiom_TCP_Accept (fst (projT1 r)) (snd (projT1 r)) skt :: tr)).
+
+Module TCP.
+
+  Definition Accept := axiom_TCP_Accept.
+
+  Definition listenSocket := axiom_TCP_listenSocket.
+  Definition bindSocket := axiom_TCP_bindSocket.
+  Definition accept : forall (skt : SockAddr) 
+    (fd : File (ListenSocketModel skt) (R :: nil)) (tr : [Trace]),
+    STsep (tr ~~ traced tr)
+          (fun r:rt => tr ~~ handle (projT2 r) *
+              traced (Accept (fst (projT1 r)) (snd (projT1 r)) skt :: tr)) :=
+      axiom_TCP_accept.
+
+End TCP.
+
+(** SSL Sockets **)
+Axiom axiom_SslListenSocketModel : SockAddr -> fd_model.
+Definition SslListenSocketModel := axiom_SslListenSocketModel.
+
+Axiom axiom_SSL_secure : forall (m : fd_model) (ms : list mode), File m ms -> Prop.
+Definition secure := axiom_SSL_secure.
+
+Axiom axiom_SSL_listenSocket : forall (skt : SockAddr),
+  STsep (__)
+        (fun fd:(File (SslListenSocketModel skt) (R :: nil)) => handle fd * [secure fd]).
+
+Axiom axiom_SSL_bindSocket : forall (local remote : SockAddr),
+  STsep (__)
+        (fun fd:File (BoundSocketModel local remote) (R :: W :: nil) => handle fd * [secure fd]).
+
+Axiom axiom_SSL_accept : forall (skt : SockAddr) (fd : File (SslListenSocketModel skt) (R :: nil))
+  (tr : [Trace]),
+  STsep (tr ~~ traced tr * [secure fd])
+        (fun r:rt => tr ~~ handle (projT2 r) * [secure fd] * [secure (projT2 r)] *
+            traced (axiom_TCP_Accept (fst (projT1 r)) (snd (projT1 r)) skt :: tr)).
+
+Module SSL.
+
+  Definition listenSocket := axiom_SSL_listenSocket.
+  Definition bindSocket := axiom_SSL_bindSocket.
+  Definition accept : forall (skt : SockAddr) 
+    (fd : File (SslListenSocketModel skt) (R :: nil)) (tr : [Trace]),
+    STsep (tr ~~ traced tr * [secure fd])
+          (fun r:rt => tr ~~ handle (projT2 r) * [secure fd] * [secure (projT2 r)] *
+              traced (TCP.Accept (fst (projT1 r)) (snd (projT1 r)) skt :: tr)) :=
+      axiom_SSL_accept.
+
+End SSL.
